wip heapletwise hyps automation

bedrock2/src/bedrock2/HeapletwiseHyps.v
@@ -5,146 +5,11 @@ Require Import coqutil.Tactics.fwd.
 Require Import coqutil.Tactics.Tactics.
 Require Import bedrock2.Lift1Prop.
 Require Import bedrock2.Map.DisjointUnion.
+Require Import bedrock2.Map.SeparationLogic.
 
 Section HeapletwiseHyps.
-  Context{key value: Type} {mem: map.map key value} {mem_ok: map.ok mem}
-    {key_eqb: key -> key -> bool} {key_eqb_spec: EqDecider key_eqb}.
-
-  (* like sep, but using disjoint union instead of map.split *)
-  Definition star(P Q: mem -> Prop)(m: mem): Prop :=
-    exists m1 m2, P m1 /\ Q m2 /\ Some m = mmap.du (Some m1) (Some m2).
-
-  Lemma star_empty_r: forall P, star P (eq map.empty) = P.
-  Proof.
-    intros. extensionality m. apply propositional_extensionality.
-    unfold star. split; intros; fwd.
-    - rewrite mmap.du_empty_r in Hp2. inversion Hp2. subst. assumption.
-    - do 2 eexists. ssplit. 1: eassumption. 1: reflexivity. rewrite mmap.du_empty_r.
-      reflexivity.
-  Qed.
-
-  Fixpoint bigstar(Ps: list (mem -> Prop)): mem -> Prop :=
-    match Ps with
-    | nil => eq map.empty
-    | h :: nil => h
-    | h :: t => star h (bigstar t)
-    end.
-
-  Fixpoint bigstar'(Ps: list (mem -> Prop)): mem -> Prop :=
-    match Ps with
-    | nil => eq map.empty
-    | h :: t => star h (bigstar' t)
-    end.
-
-  Lemma bigstar_bigstar' Ps: bigstar Ps = bigstar' Ps.
-  Proof.
-    induction Ps.
-    - reflexivity.
-    - simpl (bigstar' _). rewrite <- IHPs. destruct Ps; try reflexivity.
-      simpl. symmetry. apply star_empty_r.
-  Qed.
-
-  Definition canceling(Ps: list (mem -> Prop))(oms: list (option mem)): Prop :=
-    forall m, Some m = mmap.dus oms -> bigstar Ps m.
-
-  Lemma canceling_start: forall Ps oms m,
-      Some m = mmap.dus oms ->
-      canceling Ps oms ->
-      bigstar Ps m.
-  Proof.
-    unfold canceling. intros. apply H0. apply H.
-  Qed.
-
-  Lemma canceling_done: canceling [] [].
-  Proof.
-    unfold canceling. simpl. intros. inversion H. reflexivity.
-  Qed.
-
-  Let nth n xs := hd (@None mem) (skipn n xs).
-  Let remove_nth n (xs : list (option mem)) := firstn n xs ++ tl (skipn n xs).
-
-  Lemma cancel_head: forall n Ps (P: mem -> Prop) oms mn,
-      nth n oms = Some mn ->
-      P mn ->
-      canceling Ps (remove_nth n oms) ->
-      canceling (P :: Ps) oms.
-  Proof.
-    unfold canceling. intros.
-    rewrite bigstar_bigstar'. simpl. rewrite <- bigstar_bigstar'.
-    pose proof dus_remove_nth as A. specialize A with (1 := H) (2 := H2).
-    fwd.
-    specialize H1 with (1 := Ap0).
-    unfold star. do 2 eexists. ssplit.
-    - eassumption.
-    - eassumption.
-    - simpl. assumption.
-  Qed.
-
-  Hypothesis foo: nat -> nat -> mem -> Prop.
-
-  Example test1: forall m v1 v2 v3 v4,
-      (star (foo v1 1) (star (star (foo v2 2) (foo v3 3)) (foo v4 4))) m ->
-      exists R a4 a3, star (foo a4 4) (star (foo a3 3) R) m.
-  Proof.
-    intros.
-
-    (* destruct memory hyp into separate hypotheses: *)
-    destruct H as (m1 & m2 & HM1 & HM2 & E).
-    destruct HM2 as (m23 & m4 & HM23 & HM4 & E'). rewrite E' in E. clear m2 E'.
-    destruct HM23 as (m2 & m3 & HM2 & HM3 & E'). rewrite E' in E. clear m23 E'.
-
-    do 3 eexists. move HM1 before HM2. move m before m1.
-
-(*
-  v1, v2, v3, v4 : nat
-  m, m1, m4, m2, m3 : mem
-  HM1 : foo v1 1 m1
-  HM2 : foo v2 2 m2
-  HM3 : foo v3 3 m3
-  HM4 : foo v4 4 m4
-  E : Some m = Some m1 \*/ (Some m2 \*/ Some m3 \*/ Some m4)
-  ============================
-  star (foo ?a4 4) (star (foo ?a3 3) ?R) m
-*)
-
-    (* make goal a canceling goal: *)
-    lazymatch goal with
-    | |- star ?A (star ?B ?C) ?m => change (bigstar [A; B; C] m)
-    end.
-    rewrite mmap.du_assoc in E.
-    change (Some m = mmap.dus [Some m1; Some m2; Some m3; Some m4]) in E.
-    eapply canceling_start. 1: exact E. clear E.
-
-(*
-  ============================
-  canceling [foo ?a4 4; foo ?a3 3; ?R] [Some m1; Some m2; Some m3; Some m4]
-*)
-
-    (* canceling steps: *)
-
-    eapply (cancel_head 3). 1: reflexivity. 1: eassumption. cbn.
-
-    eapply (cancel_head 2). 1: reflexivity. 1: eassumption. cbn.
-
-    (* now that all the callee's hyps are satisfied, we need to construct the frame,
-       and we use the same canceling lemma for that as well: *)
-
-    eapply (cancel_head 0 (_ :: _)). 1: reflexivity. 1: exact HM1. cbn.
-
-    eapply (cancel_head 0 nil). 1: reflexivity. 1: exact HM2. cbn.
-
-    apply canceling_done.
-  Qed.
-
-End HeapletwiseHyps.
-
-(* Print Assumptions test1.
-   only propositional_extensionality and functional_extensionality_dep *)
-
-
-Section PresentationWithSigmas.
-  Context{key value: Type} {mem: map.map key value} {mem_ok: map.ok mem}
-    {key_eqb: key -> key -> bool} {key_eqb_spec: EqDecider key_eqb}.
+  Context {key value: Type} {mem: map.map key value} {mem_ok: map.ok mem}
+          {key_eqb: key -> key -> bool} {key_eqb_spec: EqDecider key_eqb}.
 
   (* sigma type {m: mem | P m} *)
   Inductive mem_hyp(P: mem -> Prop): Type :=
@@ -155,144 +20,211 @@ Section PresentationWithSigmas.
     | mk_mem_hyp _ m _ => m
     end.
 
+  Lemma sep_assoc_eq: forall (p q r: mem -> Prop),
+      sep (sep p q) r = sep p (sep q r).
+  Proof.
+    intros. eapply iff1ToEq. eapply sep_assoc.
+  Qed.
+
   Lemma proj_mem_hyp{P: mem -> Prop}(M: mem_hyp P): P (proj_mem M).
   Proof. destruct M as (m & HM). simpl. assumption. Qed.
 
-  Definition Star(P Q: mem -> Prop)(m: mem): Prop :=
-    exists (M1: mem_hyp P) (M2: mem_hyp Q),
-      Some m = mmap.du (Some (proj_mem M1)) (Some (proj_mem M2)).
-
-  Lemma Star_empty_r: forall P, Star P (eq map.empty) = P.
+  Lemma sep_to_sep_and_sep: forall (P Q: mem -> Prop) m,
+      sep P Q m -> exists m1 m2, P m1 /\ Q m2 /\ Some m = mmap.du (Some m1) (Some m2).
   Proof.
-    intros. extensionality m. apply propositional_extensionality.
-    unfold Star. split; intros; fwd.
-    - destruct M2 as (m2 & HM2). subst m2. simpl in H. rewrite map.du_empty_r in H.
-      inversion H. subst. destruct M1 as (m1 & HM1). simpl. assumption.
-    - unshelve (do 2 eexists).
-      + econstructor. eassumption.
-      + econstructor. reflexivity.
-      + simpl. rewrite map.du_empty_r. reflexivity.
+    unfold sep, map.split. intros. fwd. do 2 eexists. ssplit.
+    1,2: eassumption.
+    simpl. unfold map.du. eapply map.disjointb_spec in Hp0p1. rewrite Hp0p1.
+    reflexivity.
   Qed.
 
-  Fixpoint bigStar(Ps: list (mem -> Prop)): mem -> Prop :=
-    match Ps with
-    | nil => eq map.empty
-    | h :: nil => h
-    | h :: t => Star h (bigStar t)
-    end.
-
-  Fixpoint bigStar'(Ps: list (mem -> Prop)): mem -> Prop :=
-    match Ps with
-    | nil => eq map.empty
-    | h :: t => Star h (bigStar' t)
-    end.
-
-  Lemma bigStar_bigStar' Ps: bigStar Ps = bigStar' Ps.
+  Lemma sep_to_mem_hyp_and_sep: forall (P Q: mem -> Prop) m,
+      sep P Q m ->
+      exists (M1: mem_hyp P) m2, Q m2 /\ Some m = mmap.du (Some (proj_mem M1)) (Some m2).
   Proof.
-    induction Ps.
-    - reflexivity.
-    - simpl (bigStar' _). rewrite <- IHPs. destruct Ps; try reflexivity.
-      simpl. symmetry. apply Star_empty_r.
+    unfold sep, map.split. intros. fwd. unshelve eexists.
+    1: econstructor; eassumption.
+    eexists. split. 1: eassumption.
+    simpl. unfold map.du. eapply map.disjointb_spec in Hp0p1. rewrite Hp0p1.
+    reflexivity.
   Qed.
 
-  Definition Canceling(Ps: list (mem -> Prop))(oms: list (option mem)): Prop :=
-    forall m, Some m = mmap.dus oms -> bigStar Ps m.
-
-  Lemma Canceling_start: forall Ps oms m,
-      Some m = mmap.dus oms ->
-      Canceling Ps oms ->
-      bigStar Ps m.
+  Lemma sep_to_sep_and_mem_hyp: forall (P Q: mem -> Prop) m,
+      sep P Q m ->
+      exists m1 (M2: mem_hyp Q), P m1 /\ Some m = mmap.du (Some m1) (Some (proj_mem M2)).
   Proof.
-    unfold Canceling. intros. apply H0. apply H.
+    unfold sep, map.split. intros. fwd.
+    eexists. unshelve eexists.
+    1: econstructor; eassumption.
+    split. 1: eassumption.
+    simpl. unfold map.du. eapply map.disjointb_spec in Hp0p1. rewrite Hp0p1.
+    reflexivity.
   Qed.
 
-  Lemma Canceling_done: Canceling [] [].
+  Lemma sep_to_mem_hyp_and_mem_hyp: forall (P Q: mem -> Prop) m,
+      sep P Q m ->
+      exists (M1: mem_hyp P) (M2: mem_hyp Q),
+        Some m = mmap.du (Some (proj_mem M1)) (Some (proj_mem M2)).
   Proof.
-    unfold Canceling. simpl. intros. inversion H. reflexivity.
+    unfold sep, map.split. intros. fwd. unshelve (do 2 eexists).
+    1,2: econstructor; eassumption.
+    simpl. unfold map.du. eapply map.disjointb_spec in Hp0p1. rewrite Hp0p1.
+    reflexivity.
   Qed.
 
-  Let nth n xs := hd (@None mem) (skipn n xs).
-  Let remove_nth n (xs : list (option mem)) := firstn n xs ++ tl (skipn n xs).
+  Definition canceling(Ps: list (mem -> Prop))(oms: list (option mem)): Prop :=
+    forall m, Some m = mmap.dus oms -> seps Ps m.
 
-  Lemma Cancel_head: forall n Ps (P: mem -> Prop) oms mn,
-      nth n oms = Some mn ->
+  Lemma canceling_done: canceling [] [].
+  Proof.
+    unfold canceling. simpl. intros. inversion H. unfold emp. auto.
+  Qed.
+
+  (* Separate definitions to avoid simplifying user-defined expressions that
+     use the definitions from the standard library: *)
+  Definition heaplets_hd: list (option mem) -> option mem :=
+    Eval cbv delta in (@List.hd (option mem) None).
+  Definition heaplets_tl: list (option mem) -> list (option mem) :=
+    Eval cbv delta in (@List.tl (option mem)).
+  Definition heaplets_firstn: nat -> list (option mem) -> list (option mem) :=
+    Eval cbv delta in (@List.firstn (option mem)).
+  Definition heaplets_skipn: nat -> list (option mem) -> list (option mem) :=
+    Eval cbv delta in (@List.skipn (option mem)).
+  Definition heaplets_app: list (option mem) -> list (option mem) -> list (option mem) :=
+    Eval cbv delta in (@List.app (option mem)).
+  Definition heaplets_nth(n: nat)(xs: list (option mem)): option mem :=
+    heaplets_hd (skipn n xs).
+  Definition heaplets_remove_nth(n: nat)(xs : list (option mem)): list (option mem) :=
+    heaplets_app (heaplets_firstn n xs) (heaplets_tl (heaplets_skipn n xs)).
+
+  Lemma cancel_head: forall n Ps (P: mem -> Prop) oms mn,
+      heaplets_nth n oms = Some mn ->
       P mn ->
-      Canceling Ps (remove_nth n oms) ->
-      Canceling (P :: Ps) oms.
+      canceling Ps (heaplets_remove_nth n oms) ->
+      canceling (P :: Ps) oms.
   Proof.
-    unfold Canceling. intros.
-    rewrite bigStar_bigStar'. simpl. rewrite <- bigStar_bigStar'.
+    unfold canceling. intros.
+    eapply seps_cons.
     pose proof dus_remove_nth as A. specialize A with (1 := H) (2 := H2).
     fwd.
     specialize H1 with (1 := Ap0).
-    unfold Star. unshelve (do 2 eexists).
-    - econstructor. eassumption.
-    - econstructor. eassumption.
-    - simpl. assumption.
+    unfold sep. do 2 eexists. ssplit. 2,3: eassumption.
+    unfold map.split. unfold map.du in Ap1. fwd.
+    eapply map.disjointb_spec in E. auto.
   Qed.
+End HeapletwiseHyps.
+
+Ltac reify_dus e :=
+  lazymatch e with
+  | mmap.du ?h ?t => let rt := reify_dus t in constr:(cons h rt)
+  | _ => constr:(cons e nil)
+  end.
+
+Ltac reify_seps e :=
+  lazymatch e with
+  | sep ?h ?t => let rt := reify_seps t in constr:(cons h rt)
+  | _ => constr:(cons e nil)
+  end.
+
+Ltac split_sep_step :=
+  let D := fresh "D" in
+  lazymatch goal with
+  | H: sep (sep _ _) (sep _ _) _ |- _ =>
+      eapply sep_to_sep_and_sep in H;
+      let m1 := fresh "m0" in
+      let m2 := fresh "m0" in
+      destruct H as (m1 & m2 & ? & ? & D)
+  | H: sep _ (sep _ _) _ |- _ =>
+      eapply sep_to_mem_hyp_and_sep in H;
+      let M1 := fresh "M0" in
+      let m2 := fresh "m0" in
+      destruct H as (M1 & m2 & ? & D)
+  | H: sep (sep _ _) _ _ |- _ =>
+      eapply sep_to_sep_and_mem_hyp in H;
+      let m1 := fresh "m0" in
+      let M2 := fresh "M0" in
+      destruct H as (m1 & M2 & ? & D)
+  | H: sep _ _ _ |- _ =>
+      eapply sep_to_mem_hyp_and_mem_hyp in H;
+      let M1 := fresh "M0" in
+      let M2 := fresh "M0" in
+      destruct H as (M1 & M2 & D)
+  end.
+
+Ltac merge_du_step :=
+  lazymatch reverse goal with
+  | H: Some ?m = mmap.du _ _ |- _ => rewrite H in *; clear m H
+  end.
+
+
+Section HeapletwiseHypsTests.
+  Context {key value: Type} {mem: map.map key value} {mem_ok: map.ok mem}
+          {key_eqb: key -> key -> bool} {key_eqb_spec: EqDecider key_eqb}.
 
   Hypothesis foo: nat -> nat -> mem -> Prop.
 
-  Lemma mem_hyp_Star(P Q: mem -> Prop)(MP: mem_hyp P)(MQ: mem_hyp Q)(m: mem):
-    Some m = Some (proj_mem MP) \*/ Some (proj_mem MQ) ->
-    mem_hyp (Star P Q).
-  Proof.
-    econstructor. unfold Star. exists MP, MQ. eassumption.
-  Qed.
-
-  Ltac reify_dus e :=
-    lazymatch e with
-    | mmap.du ?h ?t => let rt := reify_dus t in constr:(cons h rt)
-    | _ => constr:(cons e nil)
-    end.
-
   Goal forall m v1 v2 v3 v4 (Rest: mem -> Prop),
-      (Star (foo v1 1) (Star (Star (foo v2 2) (foo v3 3)) (foo v4 4))) m ->
-      exists R a4 a3, Star (foo a4 4) (Star (foo a3 3) R) m.
+      (sep (foo v1 1) (sep (sep (foo v2 2) (foo v3 3)) (sep (foo v4 4) Rest))) m ->
+      exists R a4 a3, sep (sep (foo a4 4) (foo a3 3)) R m.
   Proof.
     intros.
-    destruct H as (M1 & M2 & E).
-    destruct M2 as (m2 & HM2). cbn [proj_mem] in E.
-    destruct HM2 as (M2 & M4 & E2). rewrite E2 in E. clear m2 E2.
-    destruct M2 as (m2 & HM2). cbn [proj_mem] in E.
-    destruct HM2 as (M2 & M3 & E2). rewrite E2 in E. clear m2 E2.
+    repeat split_sep_step.
+    repeat merge_du_step.
 
     do 3 eexists.
 
-    (* make goal a Canceling goal: *)
+
     lazymatch goal with
-    | |- Star ?A (Star ?B ?C) ?m => change (bigStar [A; B; C] m)
+    | D: Some ?m = mmap.du _ _ |- _ ?m =>
+        rewrite ?mmap.du_assoc in D;
+        let memtree := lazymatch type of D with Some m = ?e => e end in
+        let memlist := reify_dus memtree in
+        rewrite ?sep_assoc_eq;
+        let clausetree := lazymatch goal with |- ?e m => e end in
+        let clauselist := reify_seps clausetree in
+        revert m D;
+
+        lazymatch goal with
+        | |- ?g => assert (g = canceling clauselist memlist)
+        end
+
     end.
-    rewrite mmap.du_assoc in E.
-    match type of E with
-    | Some ?m = ?e => let r := reify_dus e in change (Some m = mmap.dus r) in E
-    end.
-    eapply Canceling_start. 1: exact E. clear E.
+    {
+      unfold canceling.
+      (* simpl. (* https://github.com/coq/coq/issues/5378 ? *) *)
+      cbn [seps mmap.dus].
+      reflexivity.
+    }
+    rewrite H. clear H.
 
 (*
-  M1 : mem_hyp (foo v1 1)
-  M2 : mem_hyp (foo v2 2)
-  M3 : mem_hyp (foo v3 3)
-  M4 : mem_hyp (foo v4 4)
+  M0 : mem_hyp (foo v1 1)
+  M3 : mem_hyp (foo v2 2)
+  M4 : mem_hyp (foo v3 3)
+  M1 : mem_hyp (foo v4 4)
+  M2 : mem_hyp Rest
   ============================
-  Canceling [foo ?a4 4; foo ?a3 3; ?R]
-    [Some (proj_mem M1); Some (proj_mem M2); Some (proj_mem M3); Some (proj_mem M4)]
+  canceling [foo ?a4 4; foo ?a3 3; ?R]
+    [Some (proj_mem M0); Some (proj_mem M3); Some (proj_mem M4);
+    Some (proj_mem M1); Some (proj_mem M2)]
 *)
 
-    (* Canceling steps: *)
+    (* canceling steps: *)
 
-    eapply (Cancel_head 3). 1: reflexivity. 1: eapply proj_mem_hyp. cbn.
+    eapply (cancel_head 3). 1: reflexivity. 1: eapply proj_mem_hyp. cbn.
 
-    eapply (Cancel_head 2). 1: reflexivity. 1: eapply proj_mem_hyp. cbn.
+    eapply (cancel_head 2). 1: reflexivity. 1: eapply proj_mem_hyp. cbn.
 
     (* now that all the callee's hyps are satisfied, we need to construct the frame,
-       and we use the same Canceling lemma for that as well: *)
+       and we use the same canceling lemma for that as well: *)
 
-    eapply (Cancel_head 0 (_ :: _)). 1: reflexivity. 1: eapply proj_mem_hyp. cbn.
+    eapply (cancel_head 0 (_ :: _)). 1: reflexivity. 1: eapply proj_mem_hyp. cbn.
 
-    eapply (Cancel_head 0 nil). 1: reflexivity. 1: eapply proj_mem_hyp. cbn.
+    eapply (cancel_head 0 (_ :: _)). 1: reflexivity. 1: eapply proj_mem_hyp. cbn.
 
-    apply Canceling_done.
+    eapply (cancel_head 0 nil). 1: reflexivity. 1: eapply proj_mem_hyp. cbn.
+
+    apply canceling_done.
   Qed.
 
-End PresentationWithSigmas.
+End HeapletwiseHypsTests.
